re-defining witness/recall in MRef

ulib/FStar.MRef.fst
@@ -23,3 +23,18 @@ abstract val recall_token: #a:Type -> #b:preorder a -> m:mref a b -> p:(a -> Typ
                            -> ST unit (requires (fun _ ->  token m p))
                                      (ensures (fun h0 _ h1 -> h0==h1 /\ p (sel h1 m)))
 let recall_token #a #b m p = gst_recall (p_pred m p)
+
+
+(* KM : These don't have much to do here... *)
+
+abstract val recall: p:(heap -> Type){ST.stable p} ->
+  ST unit
+    (requires (fun _ ->  witnessed p))
+    (ensures (fun h0 _ h1 -> h0 == h1 /\ p h1))
+let recall p = gst_recall p
+
+abstract val witness: p:(heap -> Type){ST.stable p} ->
+  ST unit
+    (requires (fun h0 -> p h0))
+    (ensures (fun h0 _ h1 -> h0==h1 /\ witnessed p))
+let witness p = gst_witness p
